FEATURE bounds checking pointers
- this enforces address computations by introducing a valid_ptr
predicate and folding it into the Loc and Offset types.

theories/lang/cpp/logic/path_pred.v
@@ -8,11 +8,12 @@ Require Import Coq.NArith.BinNat.
 Require Import Coq.ZArith.BinInt.
 Require Import Coq.Strings.String.
 
+Require Import iris.proofmode.tactics.
 From iris.bi Require Export monpred.
 
 From bedrock.lang.cpp Require Import semantics logic.pred ast.
 
-Local Open Scope string_scope.
+Set Default Proof Using "Type".
 
 Lemma monPred_at_persistent_inv {V bi} (P : monPred V bi) :
   (∀ i, Persistent (P i)) → Persistent P.
@@ -23,14 +24,20 @@ Lemma monPred_at_timeless_inv {V sbi} (P : monPredSI V sbi) :
 Proof. intros HP. constructor=> i. MonPred.unseal. apply HP. Qed.
 
 Section with_Σ.
-  Context `{has_cpp : cpp_logic ti}.
+  Context `{has_cpp : cpp_logic}.
 
   (* locations are computations that produce an address.
    * - note(gmm): they are always computable from the program except.
    *)
-  Definition Loc : Type := option ptr.
+  Record Loc : Type :=
+    { _location : ptr -> mpred
+    ; _loc_unique : forall p1 p2, _location p1 ** _location p2 |-- [| p1 = p2 |]
+    ; _loc_valid : forall p1, _location p1 |-- valid_ptr p1
+    ; _loc_persist :> forall p, Persistent (_location p)
+    ; _loc_affine :> forall p, Affine (_location p)
+    }.
 
-  Definition Offset : Type := option (ptr -> option ptr).
+  Global Existing Instances _loc_persist _loc_affine.
 
   Local Ltac solve_Loc_persistent X :=
     intros;
@@ -57,7 +64,7 @@ Section with_Σ.
     apply _.
 
   Definition LocEq (l1 l2 : Loc) : Prop :=
-    l1 = l2.
+    forall p, l1.(_location) p -|- l2.(_location) p.
 
   (* ^ these two could be duplicable because regions don't need to be
    * reused. the reason that local variables need to be tracked is that
@@ -71,8 +78,19 @@ Section with_Σ.
    *)
 
   (* absolute locations *)
-  Definition _eq_def (p : ptr) : Loc :=
-    Some p.
+  Definition invalid : Loc.
+  refine
+    {| _location _ := lfalse |}.
+  abstract (intros; iIntros "[[] _]").
+  abstract (intros; iIntros "[]").
+  Defined.
+
+  Definition _eq_def (p : ptr) : Loc.
+  refine
+    {| _location p' := [| p = p' |] ** valid_ptr p' |}.
+  abstract (intros; iIntros "[[-> _] [#H _]]"; iFrame "#").
+  abstract (intros; iIntros "[-> #H]"; iFrame "#").
+  Defined.
   Definition _eq_aux : seal (@_eq_def). by eexists. Qed.
   Definition _eq := _eq_aux.(unseal).
   Definition _eq_eq : @_eq = _ := _eq_aux.(seal_eq).
@@ -80,7 +98,7 @@ Section with_Σ.
   Definition _eqv (a : val) : Loc :=
     match a with
     | Vptr p => _eq p
-    | _ => None
+    | _ => invalid
     end.
 
   Lemma _eqv_eq : forall p, _eqv (Vptr p) = _eq p.
@@ -88,8 +106,8 @@ Section with_Σ.
 
   Definition _global_def (resolve : genv) (x : obj_name) : Loc :=
     match glob_addr resolve x with
-    | None => None
-    | Some p => Some p
+    | Some p => _eq p
+    | _ => invalid
     end.
   Definition _global_aux : seal (@_global_def). by eexists. Qed.
   Definition _global := _global_aux.(unseal).
@@ -98,36 +116,61 @@ Section with_Σ.
   Definition _local (ρ : region) (b : ident) : Loc :=
     match get_location ρ b with
     | Some p => _eq p
-    | _ => None
+    | _ => invalid
     end.
 
   Definition _this (ρ : region) : Loc :=
     match get_this ρ with
     | Some p => _eq p
-    | _ => None
+    | _ => invalid
     end.
 
   Definition _result (ρ : region) : Loc :=
     match get_result ρ with
     | Some p => _eq p
-    | _ => None
+    | _ => invalid
     end.
 
-  (* offsets *)
-  Definition _field_def (resolve: genv) (f : field) : Offset :=
-    match offset_of resolve f.(f_type) f.(f_name) with
-    | Some o => Some (fun p => Some (offset_ptr_ o p))
-    | _ => None
+  (** offsets *)
+  Record Offset : Type :=
+  { _offset : ptr -> ptr -> mpred
+  ; _off_functional : forall p p1 p2, _offset p p1 ** _offset p p2 |-- [| p1 = p2 |]
+  ; _off_valid : forall p1 p2, valid_ptr p1 ** _offset p1 p2 |-- valid_ptr p2
+  ; _off_persist :> forall p1 p2, Persistent (_offset p1 p2)
+  ; _off_affine :> forall p1 p2, Affine (_offset p1 p2)
+  }.
+
+  Global Existing Instances _off_persist _off_affine.
+
+  Local Definition invalidO : Offset.
+  refine {| _offset _ _ := lfalse |}.
+  abstract (intros; iIntros "[_ []]").
+  abstract (intros; iIntros "[_ []]").
+  Defined.
+
+  Definition offsetO (o : Z) : Offset.
+  refine {| _offset from to := [| to = offset_ptr_ o from |] ** valid_ptr to |}.
+  abstract (intros; iIntros "[[#H _] [-> _]]"; iFrame "#").
+  abstract (intros; iIntros "[A [B C]]"; iFrame).
+  Defined.
+
+  Definition offsetO_opt (o : option Z) : Offset :=
+    match o with
+    | None => invalidO
+    | Some o => offsetO o
     end.
+
+  Definition _field_def (resolve: genv) (f : field) : Offset :=
+    offsetO_opt (offset_of resolve f.(f_type) f.(f_name)).
   Definition _field_aux : seal (@_field_def). Proof using. by eexists. Qed.
   Definition _field := _field_aux.(unseal).
   Definition _field_eq : @_field = _ := _field_aux.(seal_eq).
 
   Definition _sub_def (resolve:genv) (t : type) (i : Z) : Offset :=
-    match size_of resolve t with
-    | Some n => Some (fun p => Some (offset_ptr_ (i * Z.of_N n) p))
-    | _ => None
-    end.
+    offsetO_opt (match size_of resolve t with
+                 | Some o => Some (Z.of_N o * i)%Z
+                 | _ => None
+                 end).
   Definition _sub_aux : seal (@_sub_def). by eexists. Qed.
   Definition _sub := _sub_aux.(unseal).
   Definition _sub_eq : @_sub = _ := _sub_aux.(seal_eq).
@@ -136,46 +179,62 @@ Section with_Σ.
      todo: determine if this needs to handle a chain.
    *)
   Definition _super_def (resolve:genv) (sub super : globname) : Offset :=
-    match parent_offset resolve sub super with
-    | Some o => Some (fun p => Some (offset_ptr_ o p))
-    | _ => None
-    end.
+    offsetO_opt (parent_offset resolve sub super).
   Definition _super_aux : seal (@_super_def). by eexists. Qed.
   Definition _super := _super_aux.(unseal).
   Definition _super_eq : @_super = _ := _super_aux.(seal_eq).
 
-  Definition _id_def : Offset := Some (fun x => Some x).
+  Definition _id_def : Offset.
+   refine {| _offset from to := [| from = to |] |}.
+   abstract (intros; iIntros "[-> #H]"; iFrame "#").
+   abstract (intros; iIntros "[H <-]"; iFrame).
+  Defined.
   Definition _id_aux : seal (@_id_def). by eexists. Qed.
   Definition _id := _id_aux.(unseal).
   Definition _id_eq : @_id = _ := _id_aux.(seal_eq).
 
-  Definition _dot_def (o1 o2 : Offset) : Offset :=
-    match o1 , o2 with
-    | Some o1 , Some o2 => Some (fun x => match o1 x with
-                                      | None => None
-                                      | Some p => o2 p
-                                      end)
-    | _ , _ => None
-    end.
+  Definition _dot_def (o1 o2 : Offset) : Offset.
+  refine {| _offset from to :=
+              Exists mid, _offset o1 from mid ** _offset o2 mid to |}.
+  { intros.
+    iIntros "[H1 H2]".
+    iDestruct "H1" as (m1) "[A A']".
+    iDestruct "H2" as (m2) "[B B']".
+    iDestruct (_off_functional with "[A B]") as %X. iFrame.
+    subst.
+    iDestruct ((_off_functional o2) with "[A' B']") as %Y. iFrame.
+    subst. iModIntro. iStopProof. eapply bi.pure_intro. reflexivity. }
+  { intros.
+    iIntros "[H H']".
+    iDestruct "H'" as (m) "[H1 H2]".
+    iApply _off_valid. iFrame.
+    iApply _off_valid. iFrame. }
+  Defined.
   Definition _dot_aux : seal (@_dot_def). by eexists. Qed.
   Definition _dot := _dot_aux.(unseal).
   Definition _dot_eq : @_dot = _ := _dot_aux.(seal_eq).
 
-  Definition _offsetL_def (o : Offset) (l : Loc) : Loc :=
-    match o , l with
-    | Some o , Some l => match o l with
-                        | None => None
-                        | Some p => Some p
-                        end
-    | _ , _ => None
-    end.
+  Definition _offsetL_def (o : Offset) (l : Loc) : Loc.
+  refine
+    {| _location p := Exists from, _offset o from p ** _location l from |}.
+  { intros. iIntros "[L R]".
+    iDestruct "L" as (pl) "[Lo Ll]".
+    iDestruct "R" as (pr) "[Ro Rl]".
+    iDestruct ((@_loc_unique l pl pr) with "[Ll Rl]") as %H; [ iFrame | ].
+    subst.
+    iApply _off_functional. iFrame. }
+  { intros.
+    iIntros "H".
+    iDestruct "H" as (p) "[O L]".
+    iApply _off_valid. iFrame.
+    iApply _loc_valid. iFrame. }
+  Defined.
   Definition _offsetL_aux : seal (@_offsetL_def). by eexists. Qed.
   Definition _offsetL := _offsetL_aux.(unseal).
   Definition _offsetL_eq : @_offsetL = _ := _offsetL_aux.(seal_eq).
 
-
   Definition addr_of_def (a : Loc) (b : ptr) : mpred :=
-    [| a = Some b |].
+    a.(_location) b.
   Definition addr_of_aux : seal (@addr_of_def). by eexists. Qed.
   Definition addr_of := addr_of_aux.(unseal).
   Definition addr_of_eq : @addr_of = _ := addr_of_aux.(seal_eq).
@@ -183,7 +242,14 @@ Section with_Σ.
   Notation "a &~ b" := (addr_of a b) (at level 30, no associativity).
 
   Global Instance addr_of_persistent : Persistent (addr_of o l).
-  Proof. rewrite addr_of_eq. apply _. Qed.
+  Proof.
+    intros. rewrite addr_of_eq /addr_of_def. apply _loc_persist.
+  Qed.
+
+  Global Instance addr_of_affine : Affine (addr_of o l).
+  Proof.
+    intros. rewrite addr_of_eq /addr_of_def. apply _loc_affine.
+  Qed.
 
   (* this is for `Indirect` field references *)
   Fixpoint path_to_Offset (resolve:genv) (from : globname) (final : ident)
@@ -211,7 +277,7 @@ Notation "a &~ b" := (addr_of a b) (at level 30, no associativity).
 
 Global Opaque _sub _field _offsetL _dot addr_of.
 
-Arguments _super {resolve} _ _ : rename.
-Arguments _field {resolve} _ : rename.
-Arguments _sub {resolve} _ : rename.
-Arguments _global {resolve} _ : rename.
+Arguments _super {_ Σ} {resolve} _ _ : rename.
+Arguments _field {_ Σ} {resolve} _ : rename.
+Arguments _sub {_ Σ} {resolve} _ : rename.
+Arguments _global {_ Σ} {resolve} _ : rename.
