theories/lang/cpp/logic/compilation_unit.v
@@ -30,7 +30,7 @@ Section with_cpp.
 
   Set Default Proof Using "Σ resolve".
 
-  Local Notation _global := (@_global resolve) (only parsing).
+  Local Notation _global := (_global (Σ:=Σ) (resolve:=resolve)) (only parsing).
   Local Notation code_at := (@code_at _ Σ) (only parsing).
   Local Notation method_at := (@method_at _ Σ) (only parsing).
   Local Notation ctor_at := (@ctor_at _ Σ) (only parsing).
